[Progress] Finish a critical lemma for refinement and add syncedness of the disk to rep invariants.

src/Implementations/LogCache/LogCache.v
@@ -92,7 +92,8 @@ Definition cached_log_rep merged_disk (s: Language.state CachedDiskLang) :=
   exists txns,
     fst s = Mem.list_upd_batch empty_mem (map addr_list txns) (map data_blocks txns) /\
     log_rep txns (snd s) /\
-    merged_disk = total_mem_map fst (shift (plus data_start) (list_upd_batch_set (snd (snd s)) (map addr_list txns) (map data_blocks txns))).
+    merged_disk = total_mem_map fst (shift (plus data_start) (list_upd_batch_set (snd (snd s)) (map addr_list txns) (map data_blocks txns))) /\
+    (forall a, a >= data_start -> snd ((snd (snd s)) a) = []).
 
 Definition cached_log_crash_rep cached_log_crash_state (s: Language.state CachedDiskLang) :=
   match cached_log_crash_state with
@@ -100,49 +101,656 @@ Definition cached_log_crash_rep cached_log_crash_state (s: Language.state Cached
     (exists txns,
        log_crash_rep (During_Commit_Log_Write txns) (snd s) /\
        old_merged_disk = total_mem_map fst (shift (plus data_start)
-       (list_upd_batch (sync (snd (snd s))) (map addr_list txns)
-                       (map (map (fun vs => (vs, []))) (map data_blocks txns))))) \/
+       (list_upd_batch_set (snd (snd s)) (map addr_list txns) (map data_blocks txns))) /\
+       (forall a, a >= data_start -> snd ((snd (snd s)) a) = [])) \/
     (exists old_txns txns,
        log_crash_rep (During_Commit_Header_Write old_txns txns) (snd s) /\
+
        new_merged_disk = total_mem_map fst (shift (plus data_start)
-        (list_upd_batch (sync (snd (snd s))) (map addr_list txns)
-          (map (map (fun vs => (vs, []))) (map data_blocks txns)))) /\
-       old_merged_disk = total_mem_map fst (shift (plus data_start)
-        (list_upd_batch (sync (snd (snd s))) (map addr_list old_txns)
-                        (map (map (fun vs => (vs, []))) (map data_blocks old_txns)))))
+        (list_upd_batch_set (snd (snd s)) (map addr_list txns)
+           (map data_blocks txns))) /\
+
+    old_merged_disk = total_mem_map fst (shift (plus data_start)
+        (list_upd_batch_set (snd (snd s)) (map addr_list old_txns)
+                            (map data_blocks old_txns))) /\
+    (forall a, a >= data_start -> snd ((snd (snd s)) a) = []))
+      
   | After_Commit new_merged_disk =>
     exists txns,
     log_rep txns (snd s) /\
      new_merged_disk = total_mem_map fst (shift (plus data_start)
-        (list_upd_batch (sync (snd (snd s))) (map addr_list txns)
-                        (map (map (fun vs => (vs, []))) (map data_blocks txns))))
+        (list_upd_batch_set (snd (snd s)) (map addr_list txns)
+                            (map data_blocks txns))) /\
+     (forall a, a >= data_start -> snd ((snd (snd s)) a) = [])
 
   | During_Apply merged_disk =>
     exists txns,
     log_crash_rep (Log.During_Apply txns) (snd s) /\
      merged_disk = total_mem_map fst (shift (plus data_start)
-        (list_upd_batch (sync (snd (snd s))) (map addr_list txns)
-                        (map (map (fun vs => (vs, []))) (map data_blocks txns))))
+        (list_upd_batch_set (snd (snd s)) (map addr_list txns)
+                        (map data_blocks txns)))
 
   | After_Apply merged_disk =>
     log_rep [] (snd s) /\
-      merged_disk = total_mem_map fst (shift (plus data_start) (snd (snd s)))
+    merged_disk = total_mem_map fst (shift (plus data_start) (snd (snd s))) /\
+    (forall a, a >= data_start -> snd ((snd (snd s)) a) = [])
    
   | During_Recovery merged_disk =>
     exists txns,
     log_crash_rep (Log.During_Recovery txns) (snd s) /\
     merged_disk = total_mem_map fst (shift (plus data_start)
         (list_upd_batch_set (snd (snd s)) (map addr_list txns)
-                            (map data_blocks txns)))
+                            (map data_blocks txns))) /\
+    (forall a, a >= data_start -> snd ((snd (snd s)) a) = [])
     end.
 
 Definition cached_log_reboot_rep merged_disk (s: Language.state CachedDiskLang) :=
   exists txns,
     log_reboot_rep txns (snd s) /\
-    merged_disk = total_mem_map fst (shift (plus data_start) (list_upd_batch_set (snd (snd s)) (map addr_list txns) (map data_blocks txns))).
+    merged_disk = total_mem_map fst (shift (plus data_start) (list_upd_batch_set (snd (snd s)) (map addr_list txns) (map data_blocks txns))) /\
+    (forall a, a >= data_start -> snd ((snd (snd s)) a) = []).
 
 
 Set Nested Proofs Allowed.
+
+(*** LEMMAS ***)
+  Lemma upd_batch_noop:
+    forall A (AEQ: EqDec A) V (l_a: list A) (l_v: list V) m tm,
+      Mem.upd_batch m l_a l_v = m ->
+      Forall (fun a => m a = None) l_a -> 
+      length l_a = length l_v ->
+      upd_batch tm l_a l_v = tm.
+  Proof.
+    induction l_a; simpl; intros; eauto.
+    destruct l_v; eauto.
+    inversion H0; cleanup.
+    destruct (in_dec AEQ a l_a).
+    {
+      rewrite Mem.upd_batch_upd_in_noop in H; eauto.
+      rewrite upd_batch_upd_in_noop; eauto.
+    }
+    {
+      rewrite Mem.upd_batch_upd in H; eauto.
+      eapply equal_f with (x:= a) in H.              
+      rewrite Mem.upd_eq in *; eauto; cleanup.
+    }
+  Qed.
+
+  Lemma list_upd_batch_noop:
+    forall A (AEQ: EqDec A) V (l_l_a: list (list A)) (l_l_v: list (list V)) m,
+      Mem.list_upd_batch m l_l_a l_l_v = m ->
+      Forall (Forall (fun a => m a = None)) l_l_a ->
+      Forall2 (fun l_a l_v => length l_a = length l_v) l_l_a l_l_v ->
+      (forall tm, list_upd_batch tm l_l_a l_l_v = tm).
+  Proof.
+    do 4 intro.
+    eapply rev_ind with
+        (P:= fun l_l_a =>
+               forall (l_l_v : list (list V)) (m : mem),
+                 Mem.list_upd_batch m l_l_a l_l_v = m ->
+                 Forall (Forall (fun a : A => m a = None)) l_l_a ->                      
+                 Forall2 (fun l_a l_v => length l_a = length l_v) l_l_a l_l_v ->
+                 forall tm : total_mem, list_upd_batch tm l_l_a l_l_v = tm);
+    simpl; intros; eauto.
+    {
+      destruct (nil_or_app l_l_v); cleanup.
+      destruct (l++[x]); simpl; eauto.
+      
+      
+      eapply_fresh forall2_length in H2.
+      repeat rewrite app_length in *; simpl in *.
+      eapply_fresh Forall2_app_split in H2; cleanup; eauto; try lia.
+      eapply_fresh forall_app_l in H1.
+      eapply_fresh forall_app_r in H1.
+      rewrite Mem.list_upd_batch_app in H0; simpl in *; try lia.
+      inversion Hx0; cleanup.
+      rewrite list_upd_batch_app; simpl in *; try lia.
+      destruct (nil_or_app x); cleanup;
+      simpl in *; eauto.
+      destruct (nil_or_app x0); cleanup.
+      destruct (x3 ++ [x2]); simpl in *; eauto.
+      inversion H4; cleanup.
+      repeat rewrite app_length in *; simpl in *.
+      rewrite Mem.upd_batch_app in *; simpl in *; try lia.
+      apply forall_app_l in H7; inversion H7; cleanup.
+      apply equal_f with (x0:= x2) in H0.
+      rewrite Mem.upd_eq in *; eauto; cleanup.
+    }
+  Qed.
+
+  Lemma upd_batch_noop_empty_mem:
+    forall A (AEQ: EqDec A) V (l_a: list A) (l_v: list V) tm,
+      Mem.upd_batch empty_mem l_a l_v = empty_mem ->
+      length l_a = length l_v ->
+      upd_batch tm l_a l_v = tm.
+  Proof.
+    induction l_a; simpl; intros; eauto.
+    destruct l_v; eauto.
+    destruct (in_dec AEQ a l_a).
+    {
+      rewrite Mem.upd_batch_upd_in_noop in H; eauto.
+      rewrite upd_batch_upd_in_noop; eauto.
+    }
+    {
+      rewrite Mem.upd_batch_upd in H; eauto.
+      eapply equal_f with (x:= a) in H.              
+      rewrite Mem.upd_eq in *; eauto.
+      unfold empty_mem in *; congruence.
+    }
+  Qed.
+  
+  Lemma upd_batch_eq_empty_mem:
+    forall A (AEQ: EqDec A) V (l_a: list A) (l_v: list V) m,
+      Mem.upd_batch m l_a l_v = empty_mem ->
+      m = empty_mem /\
+      (l_a = [] \/ l_v = []).
+  Proof.
+    induction l_a; simpl; intros; eauto.
+    destruct l_v; eauto.
+    eapply IHl_a in H.
+    destruct H.
+    eapply equal_f with (x:=a) in H.
+    rewrite Mem.upd_eq in H; eauto.
+    unfold empty_mem in *; congruence.
+  Qed.
+
+  Lemma list_upd_batch_eq_empty_mem:
+    forall A (AEQ: EqDec A) V (l_l_a: list (list A)) (l_l_v: list (list V)) m,
+      Mem.list_upd_batch m l_l_a l_l_v = empty_mem ->
+      m = empty_mem /\
+      (forall tm, list_upd_batch tm l_l_a l_l_v = tm).
+  Proof.
+    induction l_l_a; simpl; intros; eauto.
+    destruct l_l_v; eauto.
+    eapply IHl_l_a in H.
+    destruct H.
+    apply upd_batch_eq_empty_mem in H.
+    destruct H.
+    split; eauto.
+    intros; rewrite H0.            
+    intuition; subst; simpl; eauto.
+    destruct a; eauto.
+  Qed.
+
+  Lemma skipn_eq_nil:
+    forall T (l: list T) n,
+      skipn n l = nil ->
+      l = [] \/ n >= length l.
+  Proof.
+    induction l; simpl; intros; eauto.
+    destruct n; simpl in *; eauto.
+    apply IHl in H.
+    intuition subst; simpl; try lia.
+  Qed.
+
+  Fixpoint remove_by_fst {A} {AEQ: EqDec A} {V} (a: A) (l_av: list (A * V)) :=
+    match l_av with
+    | nil => nil
+    | av :: l_av' =>
+      if (AEQ a (fst av)) then
+        remove_by_fst a l_av'
+      else
+        av :: remove_by_fst a l_av'
+    end.
+
+  Lemma remove_by_fst_not_in:
+    forall A (AEQ: EqDec A) V (l: list (A * V)) a,
+      ~ In a (map fst (remove_by_fst a l)).
+  Proof.
+    induction l; simpl; eauto.
+    intros.
+    destruct (AEQ a0 (fst a)); subst; eauto.
+    simpl; intuition eauto.
+  Qed.
+
+  Lemma remove_by_fst_incl:
+    forall A (AEQ: EqDec A) V (l: list (A * V)) a,
+      incl (remove_by_fst a l) l.
+  Proof.
+    unfold incl; induction l; simpl; intros; eauto.
+    destruct (AEQ a0 (fst a)); subst; eauto.
+    inversion H; simpl in *; intuition eauto.
+  Qed.
+  
+  Lemma upd_batch_upd_remove_by_fst:
+    forall A AEQ V l_a l_v (m: @mem A AEQ V) a v,
+    let l_av := remove_by_fst a (combine l_a l_v) in
+      Mem.upd (Mem.upd_batch m l_a l_v) a v =
+      Mem.upd (Mem.upd_batch m (map fst l_av) (map snd l_av)) a v.
+  Proof.
+    unfold incl; induction l_a; simpl; intros; eauto.
+    {
+      destruct l_v; simpl; eauto.
+      destruct (AEQ a0 a); subst.
+      rewrite IHl_a.
+      rewrite Mem.upd_batch_upd; eauto.
+      rewrite Mem.upd_repeat; eauto.
+      apply remove_by_fst_not_in.
+
+      rewrite IHl_a; simpl; intuition eauto.
+    }
+  Qed.
+
+   Lemma upd_batch_upd_remove_by_fst_total:
+    forall A AEQ V l_a l_v (m: @total_mem A AEQ V) a v,
+    let l_av := remove_by_fst a (combine l_a l_v) in
+      upd (upd_batch m l_a l_v) a v =
+      upd (upd_batch m (map fst l_av) (map snd l_av)) a v.
+  Proof.
+    unfold incl; induction l_a; simpl; intros; eauto.
+    {
+      destruct l_v; simpl; eauto.
+      destruct (AEQ a0 a); subst.
+      rewrite IHl_a.
+      rewrite upd_batch_upd; eauto.
+      rewrite upd_repeat; eauto.
+      apply remove_by_fst_not_in.
+
+      rewrite IHl_a; simpl; intuition eauto.
+    }
+  Qed.
+
+  Lemma upd_batch_dedup_by_fst:
+    forall A AEQ V l_a l_v (m: @mem A AEQ V),
+    let l_av := dedup_by_fst AEQ (combine l_a l_v) in
+    length l_a = length l_v ->
+    Mem.upd_batch m l_a l_v =
+    Mem.upd_batch m (map fst l_av) (map snd l_av).
+  Proof.
+    induction l_a; simpl; intros; eauto.
+    {
+      destruct l_v; simpl; eauto.
+      rewrite map_fst_combine.
+      destruct (in_dec AEQ a l_a); subst.
+      rewrite Mem.upd_batch_upd_in_noop; eauto.
+      simpl; eauto.
+      simpl in *; lia.
+    }
+  Qed.
+
+  Lemma upd_batch_dedup_by_fst_total:
+    forall A AEQ V l_a l_v (m: @total_mem A AEQ V),
+    let l_av := dedup_by_fst AEQ (combine l_a l_v) in
+    length l_a = length l_v ->
+    upd_batch m l_a l_v =
+    upd_batch m (map fst l_av) (map snd l_av).
+  Proof.
+    induction l_a; simpl; intros; eauto.
+    {
+      destruct l_v; simpl; eauto.
+      rewrite map_fst_combine.
+      destruct (in_dec AEQ a l_a); subst.
+      rewrite upd_batch_upd_in_noop; eauto.
+      simpl; eauto.
+      simpl in *; lia.
+    }
+  Qed.
+
+  Fixpoint flatten {A} (l_l_a: list (list A)) :=
+    match l_l_a with
+    | nil => nil
+    | l_a :: l_l_a' =>
+      l_a ++ flatten l_l_a'
+    end.
+
+  Lemma flatten_app:
+    forall A (l1 l2: list (list A)),
+      flatten (l1 ++ l2) = flatten l1 ++ flatten l2.
+  Proof.
+    induction l1; simpl; intros; eauto.
+    rewrite <- app_assoc; eauto.
+    rewrite IHl1; eauto.
+  Qed.
+
+  Lemma flatten_length_eq:
+    forall A V l1 l2,
+      Forall2 (fun (l_a0 : list A) (l_v0 : list V) => length l_a0 = length l_v0) l1 l2 ->
+      length (flatten l1) = length (flatten l2).
+  Proof.
+    induction l1; simpl; intros; eauto.
+    apply forall2_length in H; destruct l2; simpl in *; lia.
+    eapply_fresh forall2_length in H; destruct l2; simpl in *; try lia.
+    inversion H; cleanup.
+    repeat rewrite app_length.
+    erewrite IHl1; eauto; lia.
+  Qed.
+
+  Lemma list_upd_batch_to_upd_batch:
+    forall A AEQ V l_a l_v (m: @mem A AEQ V),
+    Forall2 (fun l_a l_v => length l_a = length l_v) l_a l_v ->
+    Mem.list_upd_batch m l_a l_v =
+    Mem.upd_batch m (flatten l_a) (flatten l_v).
+  Proof.
+    do 4 intro.
+    eapply rev_ind with
+        (P:= fun l_a =>
+        forall (l_v : list (list V)) (m : mem),
+  Forall2 (fun (l_a0 : list A) (l_v0 : list V) => length l_a0 = length l_v0) l_a l_v ->
+  Mem.list_upd_batch m l_a l_v = Mem.upd_batch m (flatten l_a) (flatten l_v));
+    simpl; intros; eauto.
+    {
+      eapply_fresh forall2_length in H0.
+      rewrite app_length in *; simpl in *.      
+      destruct (nil_or_app l_v); subst; simpl in *; try lia.
+      cleanup.
+      rewrite app_length in *; simpl in *.
+      eapply Forall2_app_split in H0; cleanup; try lia.
+      rewrite Mem.list_upd_batch_app; try lia.
+      simpl.
+      repeat rewrite flatten_app; simpl.
+      repeat rewrite app_nil_r.
+      rewrite Mem.upd_batch_app.
+      rewrite H; eauto; lia.
+      apply flatten_length_eq; eauto.
+    }
+  Qed.
+
+   Lemma list_upd_batch_to_upd_batch_total:
+    forall A AEQ V l_a l_v (m: @total_mem A AEQ V),
+    Forall2 (fun l_a l_v => length l_a = length l_v) l_a l_v ->
+    list_upd_batch m l_a l_v =
+    upd_batch m (flatten l_a) (flatten l_v).
+  Proof.
+    do 4 intro.
+    eapply rev_ind with
+        (P:= fun l_a =>
+        forall (l_v : list (list V)) (m : total_mem),
+  Forall2 (fun (l_a0 : list A) (l_v0 : list V) => length l_a0 = length l_v0) l_a l_v ->
+  list_upd_batch m l_a l_v = upd_batch m (flatten l_a) (flatten l_v));
+    simpl; intros; eauto.
+    {
+      eapply_fresh forall2_length in H0.
+      rewrite app_length in *; simpl in *.      
+      destruct (nil_or_app l_v); subst; simpl in *; try lia.
+      cleanup.
+      rewrite app_length in *; simpl in *.
+      eapply Forall2_app_split in H0; cleanup; try lia.
+      rewrite list_upd_batch_app; try lia.
+      simpl.
+      repeat rewrite flatten_app; simpl.
+      repeat rewrite app_nil_r.
+      rewrite upd_batch_app.
+      rewrite H; eauto; lia.
+      apply flatten_length_eq; eauto.
+    }
+  Qed.
+  
+  Lemma upd_batch_eq_upd_batch_total:
+    forall A AEQ V l_av1 l_av2 (tm: @total_mem A AEQ V) m,
+      let l_a1 := map fst l_av1 in
+      let l_a2 := map fst l_av2 in
+      let l_v1 := map snd l_av1 in
+      let l_v2 := map snd l_av2 in
+      
+      Mem.upd_batch m l_a1 l_v1 =
+      Mem.upd_batch m l_a2 l_v2 ->
+      Forall (fun a => m a = None) l_a1 ->
+      Forall (fun a => m a = None) l_a2 ->
+      NoDup l_a1 ->
+      NoDup l_a2 ->
+      upd_batch tm l_a1 l_v1 =
+      upd_batch tm l_a2 l_v2.
+  Proof.
+    induction l_av1; simpl; intros.
+    { (** l_av1 = [] **)
+      symmetry in H; eapply upd_batch_noop in H; eauto.
+      repeat rewrite map_length; eauto.
+    }
+    (** l_av1 = a::l **)
+    inversion H0; cleanup; clear H0.
+    inversion H2; cleanup; clear H2.
+    destruct l_av2; subst; simpl in *.
+    {(** l_a2 = [] **)
+      rewrite Mem.upd_batch_upd in *; eauto.
+      eapply equal_f with (x:= fst a) in H.
+      rewrite Mem.upd_eq in *; eauto; cleanup.
+    }
+    {(** l_a2 = a'::l' **)            
+      inversion H1; cleanup; clear H1.
+      inversion H3; cleanup; clear H3.
+      destruct a, p; simpl in *.
+      destruct (AEQ a a0); subst.
+      {(** a = a0 **)
+        assert_fresh (v = v0). {
+          apply equal_f with (x:= a0) in H.                
+          do 2 rewrite Mem.upd_batch_upd in *; eauto.
+          do 2 rewrite Mem.upd_eq in *; eauto; congruence.
+        }
+        subst.
+        eapply IHl_av1; eauto.
+        {
+          eapply Forall_forall; intros; intuition.
+          destruct (AEQ a0 x); subst; intuition.
+          rewrite Mem.upd_ne; eauto.
+          eapply Forall_forall in H7; eauto.
+        }
+        {
+          eapply Forall_forall; intros; intuition.
+          destruct (AEQ a0 x); subst; intuition.
+          rewrite Mem.upd_ne; eauto.
+          eapply Forall_forall in H9; eauto.
+        }
+      }
+      {(** a <> a0 **)
+        destruct (in_dec AEQ a (map fst l_av2)).
+        {(** In a (map fst l_av2) **)
+          eapply_fresh in_map_iff in i; cleanup.
+          eapply_fresh in_split in H1; eauto; cleanup.
+          repeat rewrite map_app in *; simpl in *.
+          rewrite Mem.upd_batch_app in H; eauto.
+          rewrite upd_batch_app.
+          simpl in *.
+          assert_fresh (v = snd x). {
+            do 2 rewrite Mem.upd_batch_upd in H; eauto.
+            apply equal_f with (x2:= fst x) in H.                
+            do 2 rewrite Mem.upd_eq in *; eauto; congruence.
+            intros Hx.
+            apply NoDup_app_r in H10; inversion H10; eauto.
+          }
+          subst.
+          rewrite <- Mem.upd_batch_upd in H; eauto.
+          rewrite Mem.upd_comm in H; eauto.
+          rewrite Mem.upd_to_upd_batch_singleton with (a:= a0) in H .
+          do 2 rewrite <- Mem.upd_batch_app in H; eauto.
+          replace ([a0] ++ map fst x0 ++ map fst x1)
+            with (map fst ((a0, v0) :: x0 ++ x1)) in H.
+          replace ([v0] ++ map snd x0 ++ map snd x1)
+            with (map snd ((a0, v0) :: x0 ++ x1)) in H.
+          eapply IHl_av1 in H; eauto.
+          rewrite H.
+          simpl.
+          rewrite <- upd_batch_upd; eauto.
+          rewrite upd_comm.
+          repeat rewrite map_app;
+          rewrite upd_batch_app; eauto.
+          all: try solve [repeat rewrite map_length; eauto].
+          all: try solve [simpl; repeat rewrite map_app; eauto].
+          {
+            eapply NoDup_remove_2 in H10.
+            intros Hx; apply H10.
+            apply in_app_iff; eauto.
+          }
+          {
+            eapply Forall_forall; intros.
+            eapply Forall_forall in H7; eauto.
+            destruct (AEQ x2 (fst x)); subst; intuition.
+            rewrite Mem.upd_ne; eauto.
+          }
+          {
+            simpl.
+            eapply NoDup_remove_2 in H10.
+            constructor; eauto.
+            rewrite Mem.upd_ne; eauto.
+            rewrite map_app; simpl.
+            apply Forall_forall; intros.
+            destruct (AEQ x2 (fst x)); subst; intuition.
+            rewrite Mem.upd_ne; eauto.
+            eapply Forall_forall in H9; eauto.
+            apply in_app_iff in H0.
+            apply in_app_iff; simpl; intuition eauto.
+          }
+          {
+            eapply NoDup_remove_1 in H10.
+            simpl; rewrite map_app; constructor; eauto.
+            
+            intros Hx; apply H2.
+            apply in_app_iff in Hx.
+            apply in_app_iff; simpl; intuition eauto.
+          }
+          {
+            eapply NoDup_remove_2 in H10.
+            intros Hx; apply H10.
+            apply in_app_iff; eauto.
+          }
+        }
+        {(** ~In a (map fst l_av2) **)
+          eapply equal_f with (x:= a) in H.
+          do 2 rewrite Mem.upd_batch_ne in H; eauto.
+          rewrite Mem.upd_eq in H; eauto.
+          rewrite Mem.upd_ne in H; eauto; cleanup.
+        }
+      }
+    }
+  Qed.
+
+  Lemma in_dedup_by_fst:
+      forall A AEQ B (l: list (A * B)) ab,
+        In ab (dedup_by_fst AEQ l) ->
+        In ab l.
+    Proof.
+      induction l; simpl; intros; eauto.
+      destruct (in_dec AEQ (fst a) (map fst l)); eauto.
+      inversion H; subst; eauto.
+    Qed.
+
+    
+    Lemma in_flatten:
+      forall A (l_l_a: list (list A)) a,
+        In a (flatten l_l_a) ->
+        exists l_a, In l_a l_l_a /\ In a l_a.
+    Proof.
+      induction l_l_a; simpl; intros; eauto.
+      intuition.
+      apply in_app_iff in H; intuition eauto.
+      apply IHl_l_a in H0; destruct H0; intuition eauto.
+    Qed.
+
+          Lemma NoDup_map_fst_dedup_by_fst:
+        forall A AEQ B (l:list (A * B)),
+          NoDup (map fst (dedup_by_fst AEQ l)).
+      Proof.
+        induction l; simpl; intros; eauto.
+        constructor.
+        destruct (in_dec AEQ (fst a) (map fst l)); eauto.
+        simpl; constructor; eauto.
+        intros Hx.
+        apply in_map_iff in Hx; cleanup.
+        apply in_dedup_by_fst in H0; eauto.
+        rewrite <- H in *.
+        apply n; apply in_map; eauto.
+      Qed.
+
+
+  Lemma list_upd_batch_eq_list_upd_batch_total:
+    forall A AEQ V l_a1 l_v1 l_a2 l_v2 (tm: @total_mem A AEQ V) m,
+      Mem.list_upd_batch m l_a1 l_v1 =
+      Mem.list_upd_batch m l_a2 l_v2 ->
+      Forall (Forall (fun a => m a = None)) l_a1 ->
+      Forall (Forall (fun a => m a = None)) l_a2 ->
+      Forall2 (fun l_a l_v => length l_a = length l_v) l_a1 l_v1 ->
+      Forall2 (fun l_a l_v => length l_a = length l_v) l_a2 l_v2 ->
+      list_upd_batch tm l_a1  l_v1 =
+      list_upd_batch tm l_a2 l_v2.
+  Proof.
+    intros.
+    do 2 rewrite list_upd_batch_to_upd_batch in *; eauto.
+    setoid_rewrite list_upd_batch_to_upd_batch_total; eauto.
+    setoid_rewrite upd_batch_dedup_by_fst_total.
+    eapply upd_batch_eq_upd_batch_total; eauto.            
+    repeat rewrite <- upd_batch_dedup_by_fst; eauto.
+    all: try solve [eapply flatten_length_eq; eauto].
+    apply Forall_forall; intros.
+    apply in_map_iff in H4; cleanup.
+    apply in_dedup_by_fst in H5.
+    destruct x0; simpl in *;
+    apply in_combine_l in H5.
+    apply in_flatten in H5; cleanup.
+    eapply Forall_forall in H0; eauto.
+    eapply Forall_forall in H0; eauto.
+
+    apply Forall_forall; intros.
+    apply in_map_iff in H4; cleanup.
+    apply in_dedup_by_fst in H5.
+    destruct x0; simpl in *;
+    apply in_combine_l in H5.
+    apply in_flatten in H5; cleanup.
+    eapply Forall_forall in H1; eauto.
+    eapply Forall_forall in H1; eauto.
+
+    apply NoDup_map_fst_dedup_by_fst.
+    apply NoDup_map_fst_dedup_by_fst. 
+  Qed.
+  
+  Lemma empty_mem_list_upd_batch_eq_list_upd_batch_total:
+    forall A AEQ V l_a1 l_v1 l_a2 l_v2 (tm: @total_mem A AEQ V),
+      Mem.list_upd_batch empty_mem l_a1 l_v1 =
+      Mem.list_upd_batch empty_mem l_a2 l_v2 ->
+      Forall2 (fun l_a l_v => length l_a = length l_v) l_a1 l_v1 ->
+      Forall2 (fun l_a l_v => length l_a = length l_v) l_a2 l_v2 ->
+      list_upd_batch tm l_a1  l_v1 =
+      list_upd_batch tm l_a2 l_v2.
+  Proof.
+    intros.
+    eapply list_upd_batch_eq_list_upd_batch_total; eauto.
+    eapply Forall_forall; intuition.
+    eapply Forall_forall; intuition.
+    eapply Forall_forall; intuition.
+    eapply Forall_forall; intuition.
+  Qed.
+
+
+  
+    Lemma upd_batch_in_some_total_mem :
+      forall A AEQ V l_a l_v (m: @mem A AEQ V) (tm: @total_mem A AEQ V) a v,
+        Mem.upd_batch m l_a l_v a = Some v ->
+        m a = None ->
+        NoDup l_a ->
+        upd_batch tm l_a l_v a = v.
+    Proof.
+      induction l_a; simpl; intros; try congruence.
+      destruct l_v; simpl; try congruence.
+      destruct (AEQ a a0); subst.
+      inversion H1; cleanup.
+      rewrite upd_batch_upd; eauto.
+      rewrite Mem.upd_batch_upd in H; eauto.
+      rewrite Mem.upd_eq in H; eauto.
+      rewrite upd_eq; eauto.
+      congruence.
+      eapply IHl_a; eauto.
+      rewrite Mem.upd_ne; eauto.
+      inversion H1; eauto.
+    Qed.
+
+    Lemma log_rep_forall2_txns_length_match:
+    forall txns s,
+      log_rep txns s ->
+      Forall2 (fun l_a l_v => length l_a = length l_v)
+              (map addr_list txns) (map data_blocks txns).
+  Proof.
+    intros.
+    unfold log_rep, log_rep_general, log_rep_explicit,
+    log_rep_inner, txns_valid in *; cleanup.
+    eapply forall_forall2.
+    rewrite <- combine_map.
+    apply Forall_forall; intros.
+    apply in_map_iff in H; cleanup.
+    simpl.
+    eapply Forall_forall in H7; eauto.
+    unfold txn_well_formed in *; cleanup; eauto.
+    rewrite firstn_length_l; eauto.
+    repeat rewrite map_length; eauto.
+  Qed.
+
 
 
 (*** SPECS ***)
@@ -225,34 +833,25 @@ Proof.
     
     eapply equal_f in H.
     rewrite H in H7.
-    eapply Mem.list_upd_batch_some in H7.
-    unfold empty_mem in *; split_ors; try congruence.
     
     eexists.
     rewrite total_mem_map_shift_comm.
     rewrite shift_some.
     rewrite total_mem_map_fst_list_upd_batch_set.
     intuition eauto.
-    (** we need a connection between mem and total mem. **)
-    admit.
-    destruct s; simpl; eauto.
-    repeat rewrite map_length; eauto.
     {
-      eapply forall_forall2.
-      apply Forall_forall; intros.
-      rewrite <- combine_map in H1.
-      apply in_map_iff in H1; cleanup; simpl.
-
-      unfold log_rep, log_rep_general, log_rep_explicit in *;
-      simpl in *; logic_clean.
-      unfold log_rep_inner, txns_valid in *; logic_clean.
+      left; eexists; intuition eauto.
+      rewrite list_upd_batch_to_upd_batch in H7.
+      rewrite list_upd_batch_to_upd_batch_total.
+      rewrite upd_batch_dedup_by_fst in H7.
+      rewrite upd_batch_dedup_by_fst_total.
       
-      eapply Forall_forall in H10; eauto.
-      unfold txn_well_formed in H10; logic_clean.
-      rewrite H13 in *.
-      apply firstn_length_l; eauto; lia.
-      repeat rewrite map_length; eauto.
+      symmetry; eapply upd_batch_in_some_total_mem; eauto.
+      apply NoDup_map_fst_dedup_by_fst.
+      all: try apply flatten_length_eq.
+      all: eapply log_rep_forall2_txns_length_match; eauto.
     }
+    destruct s; simpl; eauto.
   }
 
   {
@@ -270,7 +869,6 @@ Proof.
     unfold total_mem_map; simpl.
     simpl in *; intuition eauto.
     repeat cleanup_pairs; eauto.
-    destruct s1; eauto.
     {
     eapply forall_forall2.
     apply Forall_forall; intros.
@@ -281,18 +879,16 @@ Proof.
      simpl in *; logic_clean.
      unfold log_rep_inner, txns_valid in *; logic_clean.
      
-     eapply Forall_forall in H11; eauto.
-     unfold txn_well_formed in H11; logic_clean.
-     rewrite H14 in *.
+     eapply Forall_forall in H12; eauto.
+     unfold txn_well_formed in H12; logic_clean.
+     rewrite H15 in *.
      apply firstn_length_l; eauto; lia.
      repeat rewrite map_length; eauto.
     }
   }
   intuition eauto.
   right; split; eauto; lia.
-  Unshelve.
-  exact empty_mem.
-Admitted.
+Qed.
 
 Theorem read_crashed:
   forall a s o s' u,
@@ -316,8 +912,8 @@ Lemma recover_finished:
 Proof.
   unfold recover, cached_log_reboot_rep; intros; cleanup.
   repeat invert_exec.
-  eapply recover_finished in H5; eauto.
-  apply write_lists_to_cache_finished in H3.
+  eapply recover_finished in H6; eauto.
+  apply write_lists_to_cache_finished in H4.
   repeat cleanup_pairs.
   unfold cached_log_rep; simpl; eexists; intuition eauto.
   rewrite map_fst_combine, map_snd_combine by (repeat rewrite map_length; eauto); eauto.
@@ -329,9 +925,9 @@ Proof.
     rewrite map_noop; eauto.
     intros.
     unfold log_rep, log_rep_general, log_rep_explicit, log_rep_inner, txns_valid in *; simpl in *; cleanup.
-    eapply Forall_forall in H11; eauto.
-    unfold txn_well_formed in H11; simpl in *; cleanup.
-    eapply Forall_forall in H15; eauto; lia.
+    eapply Forall_forall in H12; eauto.
+    unfold txn_well_formed in H12; simpl in *; cleanup.
+    eapply Forall_forall in H16; eauto; lia.
   }
   rewrite A at 2.
   rewrite shift_list_upd_batch_set_comm.
@@ -351,7 +947,7 @@ Proof.
     intros; lia.
   }
   {
-    intros; apply H7; lia.
+    intros; apply H8; lia.
   }
   {
     unfold sumbool_agree; intros; intuition eauto.
@@ -360,13 +956,16 @@ Proof.
     destruct (addr_dec (data_start + x0) (data_start + y)); eauto; lia.
   }
   {
+    rewrite H8; simpl; eauto.
+  }
+  {
     cleanup.
     rewrite Forall_forall; intros.
     rewrite <- combine_map in H1.
     apply in_map_iff in H1; cleanup; simpl.
     unfold log_rep, log_rep_general, log_rep_explicit, log_rep_inner, txns_valid in *; simpl in *; cleanup.
-    eapply Forall_forall in H14; eauto.
-    unfold txn_well_formed in H14; simpl in *; cleanup.
+    eapply Forall_forall in H15; eauto.
+    unfold txn_well_formed in H15; simpl in *; cleanup.
     apply firstn_length_l; eauto.
   }
 Qed.
@@ -388,7 +987,7 @@ Proof.
   intuition eauto.
   split_ors; cleanup; repeat invert_exec.
   {
-    eapply recover_crashed in H4; eauto.
+    eapply recover_crashed in H5; eauto.
     repeat cleanup_pairs.
     split_ors; cleanup.
     {
@@ -402,9 +1001,9 @@ Proof.
     rewrite map_noop; eauto.
     intros.
     unfold log_reboot_rep, log_rep_general, log_rep_explicit, log_rep_inner, txns_valid in *; simpl in *; cleanup.
-    eapply Forall_forall in H21; eauto.
-    unfold txn_well_formed in H21; simpl in *; cleanup_no_match.
-    eapply Forall_forall in H24; eauto; lia.
+    eapply Forall_forall in H22; eauto.
+    unfold txn_well_formed in H22; simpl in *; cleanup_no_match.
+    eapply Forall_forall in H25; eauto; lia.
       }
       rewrite A at 2.
       rewrite shift_list_upd_batch_set_comm.
@@ -429,6 +1028,9 @@ Proof.
         destruct (addr_dec (data_start + y) (data_start + y)); eauto; congruence.
         destruct (addr_dec (data_start + x0) (data_start + y)); eauto; lia.
       }
+      {
+        rewrite H1; eauto.
+      }
     }
     split_ors; cleanup.
     {
@@ -445,9 +1047,9 @@ Proof.
         intros.
         unfold log_reboot_rep, log_rep_general, log_rep_explicit,
         log_rep_inner, txns_valid in *; simpl in *; cleanup.
-        eapply Forall_forall in H12; eauto.
-        unfold txn_well_formed in H12; simpl in *; cleanup_no_match.
-        eapply Forall_forall in H16; eauto; lia.
+        eapply Forall_forall in H13; eauto.
+        unfold txn_well_formed in H13; simpl in *; cleanup_no_match.
+        eapply Forall_forall in H17; eauto; lia.
       }
       rewrite A at 2.
       rewrite shift_list_upd_batch_set_comm.
@@ -473,6 +1075,9 @@ Proof.
         destruct (addr_dec (data_start + y) (data_start + y)); eauto; congruence.
         destruct (addr_dec (data_start + x0) (data_start + y)); eauto; lia.
       }
+      {
+        rewrite H1; eauto.
+      }
     }
     intuition eauto.
     left; eexists; intuition eauto.
@@ -492,9 +1097,9 @@ Proof.
       intros.
       unfold log_rep, log_rep_general, log_rep_explicit,
       log_rep_inner, txns_valid in *; simpl in *; cleanup.
-      eapply Forall_forall in H11; eauto.
-      unfold txn_well_formed in H11; simpl in *; cleanup_no_match.
-      eapply Forall_forall in H15; eauto; lia.
+      eapply Forall_forall in H12; eauto.
+      unfold txn_well_formed in H12; simpl in *; cleanup_no_match.
+      eapply Forall_forall in H16; eauto; lia.
     }
     
     rewrite A at 2.
@@ -523,11 +1128,14 @@ Proof.
       destruct (addr_dec x0 y); subst.
       destruct (addr_dec (data_start + y) (data_start + y)); eauto; congruence.
       destruct (addr_dec (data_start + x0) (data_start + y)); eauto; lia.
-    } 
+    }
+    {
+      rewrite H1; simpl; eauto.
+    }
   }
   {
-    eapply Log.Specs.recover_finished in H5; eauto; cleanup.
-    apply write_lists_to_cache_crashed in H3; cleanup.
+    eapply Log.Specs.recover_finished in H6; eauto; cleanup.
+    apply write_lists_to_cache_crashed in H4; cleanup.
     repeat cleanup_pairs.
     {
       intuition eauto.
@@ -546,19 +1154,16 @@ Proof.
         intros.
         unfold log_rep, log_rep_general, log_rep_explicit,
         log_rep_inner, txns_valid in *; simpl in *; cleanup_no_match.
-        eapply Forall_forall in H12; eauto.
-        unfold txn_well_formed in H12; simpl in *; cleanup_no_match.
-        eapply Forall_forall in H23; eauto; lia.
+        eapply Forall_forall in H13; eauto.
+        unfold txn_well_formed in H13; simpl in *; cleanup_no_match.
+        eapply Forall_forall in H24; eauto; lia.
       }
     
-      rewrite <- sync_list_upd_batch_set.
-      rewrite <- sync_shift_comm.
       rewrite A at 2.
       rewrite shift_list_upd_batch_set_comm.
       rewrite shift_eq_after with (m1:=s3)(m2:=sync s4).
       rewrite <- shift_list_upd_batch_set_comm.
       rewrite <- A; eauto.
-      rewrite total_mem_map_fst_sync_noop.
       repeat rewrite total_mem_map_shift_comm.
       repeat rewrite total_mem_map_fst_list_upd_batch_set.
       rewrite total_mem_map_fst_sync_noop; eauto.
@@ -573,7 +1178,7 @@ Proof.
         intros; lia.
       }
       {
-        intros; apply H7; lia.
+        intros; apply H8; lia.
       }
       {
         unfold sumbool_agree; intros; intuition eauto.
@@ -582,6 +1187,9 @@ Proof.
         destruct (addr_dec (data_start + x9) (data_start + y)); eauto; lia.
       }
     }
+    {
+      rewrite H8; simpl; eauto.
+    }
     }
     {
       apply Forall_forall; intros.
@@ -589,9 +1197,9 @@ Proof.
       apply in_map_iff in H1; cleanup; simpl.
       unfold log_reboot_rep, log_rep_explicit, log_rep_inner, txns_valid in H;
       simpl in *; logic_clean.
-      eapply Forall_forall in H15; eauto.
-      unfold txn_well_formed in H15; logic_clean.
-      rewrite H18.
+      eapply Forall_forall in H16; eauto.
+      unfold txn_well_formed in H16; logic_clean.
+      rewrite H19.
       apply firstn_length_l; eauto.
       lia.
     }
@@ -627,9 +1235,9 @@ Proof.
     
     unfold log_rep, log_rep_general, log_rep_explicit,
     log_rep_inner, txns_valid in *; cleanup; simpl in *.
-    eapply_fresh forall_app_l in H11. 
+    eapply_fresh forall_app_l in H12. 
     inversion Hx; simpl in *; cleanup.
-    unfold txn_well_formed in H20; cleanup.
+    unfold txn_well_formed in H21; cleanup.
     rewrite firstn_app2; eauto.
     simpl; intuition eauto.
     {
@@ -652,9 +1260,9 @@ Proof.
         setoid_rewrite map_ext_in.
         apply map_id.
         intros; simpl.
-        eapply Forall_forall in H11; eauto.
-        unfold txn_well_formed in H11; logic_clean.
-        eapply Forall_forall in H34; eauto; lia.
+        eapply Forall_forall in H12; eauto.
+        unfold txn_well_formed in H12; logic_clean.
+        eapply Forall_forall in H35; eauto; lia.
         
       }
       setoid_rewrite A.
@@ -684,7 +1292,7 @@ Proof.
         destruct (addr_dec (data_start + x) (data_start + y)); eauto; lia.
       }
       {
-        apply H10; lia.
+        apply H11; lia.
       }
       {
         unfold sumbool_agree; intros; intuition eauto.
@@ -693,6 +1301,9 @@ Proof.
         destruct (addr_dec (data_start + x) (data_start + y)); eauto; lia.
       }
     }
+    {
+      rewrite H11; simpl; eauto.
+    }
     rewrite map_length; eauto.
     rewrite map_length; eauto.
   }
@@ -700,13 +1311,13 @@ Proof.
     repeat invert_exec.
     simpl in *.
     repeat cleanup_pairs; simpl in *.
-    eapply apply_log_finished in H9; eauto.
+    eapply apply_log_finished in H10; eauto.
     logic_clean.
     apply write_batch_to_cache_finished in H1.
     logic_clean.
     unfold log_rep in *; logic_clean.
-    eapply commit_finished in H10; eauto.
-    all: try rewrite H6.
+    eapply commit_finished in H11; eauto.
+    all: try rewrite H7.
     split_ors; cleanup_no_match.
     {(** second commit is success **)
     right.
@@ -717,7 +1328,7 @@ Proof.
     
     unfold log_rep, log_rep_general, log_rep_explicit,
     log_rep_inner, txns_valid in *; cleanup; simpl in *. 
-    inversion H14; simpl in *; cleanup.
+    inversion H15; simpl in *; cleanup.
     unfold txn_well_formed in H2; cleanup.
     rewrite firstn_app2; eauto.
     unfold log_header_block_rep in *; simpl in *; cleanup.
@@ -727,10 +1338,10 @@ Proof.
     }
     {
       rewrite shift_upd_batch_set_comm.
-      setoid_rewrite shift_eq_after with (m1:= s2) (m2:= sync
+      setoid_rewrite shift_eq_after with (m1:= s1) (m2:= sync
           (sync
-             (upd_set (list_upd_batch_set s0 (map addr_list x4) (map data_blocks x4)) hdr_block_num
-                      (encode_header (update_hdr (decode_header (fst (s0 hdr_block_num))) header_part0))))); intros; try lia.
+             (upd_set (list_upd_batch_set s4 (map addr_list x4) (map data_blocks x4)) hdr_block_num
+                      (encode_header (update_hdr (decode_header (fst (s4 hdr_block_num))) header_part0))))); intros; try lia.
       rewrite sync_idempotent.
       rewrite total_mem_map_fst_upd_batch_set.
       repeat rewrite total_mem_map_shift_comm.
@@ -745,7 +1356,7 @@ Proof.
         lia.
       }
       {
-        eapply H12; lia.
+        eapply H13; lia.
       }
       {
         unfold sumbool_agree; intros; intuition eauto.
@@ -754,16 +1365,19 @@ Proof.
         destruct (addr_dec (data_start + x0) (data_start + y)); eauto; lia.
       }
     }
+    {
+      rewrite H13; simpl; eauto.
+    }
     rewrite map_length; eauto.
     }
     {
-      rewrite app_length in H10.
+      rewrite app_length in H11.
       repeat cleanup_pairs.
       unfold log_rep, log_rep_general, log_rep_explicit,
       log_rep_inner, header_part_is_valid, txns_valid in *;
       simpl in *; cleanup; simpl in *. 
           
-      rewrite <- H11 in *; simpl in *.
+      rewrite <- H12 in *; simpl in *.
       lia.
     }
     {
@@ -775,7 +1389,7 @@ Proof.
     {
       rewrite firstn_app2; eauto.    
       apply Forall_forall; intros.
-      apply in_map_iff in H7; cleanup.
+      apply in_map_iff in H8; cleanup.
       eapply_fresh Forall_forall in f; eauto.
       pose proof data_fits_in_disk.
       split; try lia.
@@ -787,23 +1401,26 @@ Proof.
     {
       rewrite map_length; eauto.
     }
-  }
+  } 
   {
+    rewrite H7.
     rewrite firstn_app2; eauto.
     apply FinFun.Injective_map_NoDup; eauto.
     unfold FinFun.Injective; intros; lia.
     rewrite map_length; eauto.
   }
   {
+    rewrite H7.
     rewrite firstn_app2; eauto.    
     apply Forall_forall; intros.
-    apply in_map_iff in H7; cleanup_no_match.
+    apply in_map_iff in H8; cleanup_no_match.
     eapply_fresh Forall_forall in f; eauto.
     pose proof data_fits_in_disk.
     split; try lia.
     rewrite map_length; eauto.
   }
   {
+    rewrite H7.
     rewrite app_length, map_length; lia.
   }
 Qed.
@@ -825,18 +1442,20 @@ Proof.
     split_ors; cleanup; repeat invert_exec.
     {
       destruct (addr_list_to_blocks_to_addr_list (map (Init.Nat.add data_start) al)).
-      eapply commit_crashed in H3; eauto.
+      eapply commit_crashed in H4; eauto.
       {
         repeat (split_ors; cleanup);
         repeat cleanup_pairs; eauto.
         {
+          left; eexists; intuition eauto.
+        }
+        {
           right; left; unfold cached_log_crash_rep; simpl.
           left; eexists; intuition eauto.
-          rewrite <- sync_list_upd_batch_set.
-          rewrite <- sync_shift_comm.
           
           assert (A: map addr_list x =
-                     map (map (Init.Nat.add data_start)) (map (map (fun a => a - data_start)) (map addr_list x))). {
+                     map (map (Init.Nat.add data_start))
+                         (map (map (fun a => a - data_start)) (map addr_list x))). {
             repeat rewrite map_map; simpl.
             setoid_rewrite map_ext_in at 2.
             eauto.
@@ -847,9 +1466,9 @@ Proof.
             intros; simpl.
             unfold log_crash_rep, log_rep_inner, txns_valid in *; cleanup.
             
-            eapply Forall_forall in H13; eauto.
-            unfold txn_well_formed, record_is_valid in H13; logic_clean.
-            eapply Forall_forall in H18; eauto; lia.
+            eapply Forall_forall in H14; eauto.
+            unfold txn_well_formed, record_is_valid in H14; logic_clean.
+            eapply Forall_forall in H19; eauto; lia.
           }
           rewrite A.
           repeat rewrite shift_list_upd_batch_set_comm.
@@ -857,7 +1476,7 @@ Proof.
           {
             apply shift_eq_after.
             intros; lia.
-            intros; apply H3; lia.
+            intros; apply H4; lia.
           }
           {
             unfold sumbool_agree; intros; intuition eauto.
@@ -870,14 +1489,15 @@ Proof.
             destruct (addr_dec x0 y); subst.
             destruct (addr_dec (data_start + y) (data_start + y)); eauto; congruence.
             destruct (addr_dec (data_start + x0) (data_start + y)); eauto; lia.
+          }
+          {
+            rewrite H4; eauto.
           }
         }
         {
           right; left; unfold cached_log_crash_rep; simpl.
           right; do 2 eexists; intuition eauto.
           {
-            rewrite <- sync_list_upd_batch_set.
-            rewrite <- sync_shift_comm.
             
             assert (A: map addr_list (x++[x0]) =
                        map (map (Init.Nat.add data_start))
@@ -893,9 +1513,9 @@ Proof.
             intros; simpl.
             unfold log_crash_rep, log_rep_inner, txns_valid in *; cleanup.
             
-            eapply Forall_forall in H19; eauto.
-            unfold txn_well_formed, record_is_valid in H19; logic_clean.
-            eapply Forall_forall in H24; eauto; lia.
+            eapply Forall_forall in H20; eauto.
+            unfold txn_well_formed, record_is_valid in H20; logic_clean.
+            eapply Forall_forall in H25; eauto; lia.
           }
           assert (A0: map addr_list x =
                       map (map (Init.Nat.add data_start))
@@ -911,9 +1531,9 @@ Proof.
             intros; simpl.
             unfold log_crash_rep, log_rep_inner, txns_valid in *; cleanup.
             
-            eapply Forall_forall in H19; eauto.
-            unfold txn_well_formed, record_is_valid in H19; logic_clean.
-            eapply Forall_forall in H24; eauto; lia.
+            eapply Forall_forall in H20; eauto.
+            unfold txn_well_formed, record_is_valid in H20; logic_clean.
+            eapply Forall_forall in H25; eauto; lia.
           }
           rewrite A, A0.
           repeat rewrite shift_list_upd_batch_set_comm.
@@ -921,15 +1541,14 @@ Proof.
           
           repeat rewrite map_app.
           rewrite list_upd_batch_set_app; simpl.
-          rewrite total_mem_map_fst_sync_noop.
           rewrite total_mem_map_fst_upd_batch_set.
           unfold log_crash_rep in *; simpl in *; logic_clean.
-          unfold log_rep_inner, txns_valid in H12; logic_clean.
-          eapply forall_app_l in H15.
+          unfold log_rep_inner, txns_valid in H13; logic_clean.
+          eapply forall_app_l in H16.
           simpl in *.
-          inversion H15; subst.
-          unfold txn_well_formed in H18; logic_clean.
-          rewrite H20, H0, H4 in *.
+          inversion H16; subst.
+          unfold txn_well_formed in H19; logic_clean.
+          rewrite H21, H0, H5 in *.
           rewrite firstn_app2.
           replace (map (fun a : nat => a - data_start) (map (Init.Nat.add data_start) al)) with al; eauto.
 
@@ -945,7 +1564,7 @@ Proof.
           
           apply shift_eq_after.
           intros; lia.
-          intros; apply H6; lia.
+          intros; apply H7; lia.
           {
             unfold sumbool_agree; intros; intuition eauto.
             destruct (addr_dec x4 y); subst.
@@ -960,8 +1579,6 @@ Proof.
           }
           }
           {
-           rewrite <- sync_list_upd_batch_set.
-           rewrite <- sync_shift_comm.
            
            assert (A0: map addr_list x =
                        map (map (Init.Nat.add data_start))
@@ -977,9 +1594,9 @@ Proof.
             intros; simpl.
             unfold log_crash_rep, log_rep_inner, txns_valid in *; cleanup.
             
-            eapply Forall_forall in H19; eauto.
-            unfold txn_well_formed, record_is_valid in H19; logic_clean.
-            eapply Forall_forall in H24; eauto; lia.
+            eapply Forall_forall in H20; eauto.
+            unfold txn_well_formed, record_is_valid in H20; logic_clean.
+            eapply Forall_forall in H25; eauto; lia.
           }
           rewrite A0.
           repeat rewrite shift_list_upd_batch_set_comm.
@@ -989,7 +1606,7 @@ Proof.
 
           apply shift_eq_after.
           intros; lia.
-          intros; apply H6; lia.
+          intros; apply H7; lia.
           {
             unfold sumbool_agree; intros; intuition eauto.
             destruct (addr_dec x4 y); subst.
@@ -1002,15 +1619,15 @@ Proof.
             destruct (addr_dec (data_start + y) (data_start + y)); eauto; congruence.
             destruct (addr_dec (data_start + x4) (data_start + y)); eauto; lia.
           }
+          }
+          {
+            rewrite H7; eauto.
           }
         }
 
         {
           right; right; left; unfold cached_log_crash_rep; simpl.
           eexists; intuition eauto.
-          
-          rewrite <- sync_list_upd_batch_set.
-          rewrite <- sync_shift_comm.
           
           assert (A: map addr_list (x++[x0]) =
                      map (map (Init.Nat.add data_start))
@@ -1027,9 +1644,9 @@ Proof.
             unfold log_rep, log_rep_general, log_rep_explicit,
             log_rep_inner, txns_valid in *; cleanup.
             
-            eapply Forall_forall in H13; eauto.
-            unfold txn_well_formed, record_is_valid in H13; logic_clean.
-            eapply Forall_forall in H24; eauto; lia.
+            eapply Forall_forall in H14; eauto.
+            unfold txn_well_formed, record_is_valid in H14; logic_clean.
+            eapply Forall_forall in H25; eauto; lia.
           }
           rewrite A.
           repeat rewrite shift_list_upd_batch_set_comm.
@@ -1041,7 +1658,6 @@ Proof.
           
           repeat rewrite map_app.
           rewrite list_upd_batch_set_app; simpl.
-          rewrite total_mem_map_fst_sync_noop.
           repeat rewrite total_mem_map_shift_comm.
           repeat rewrite total_mem_map_fst_upd_batch_set.
           repeat rewrite total_mem_map_fst_list_upd_batch_set.
@@ -1050,11 +1666,11 @@ Proof.
           unfold log_rep, log_rep_general, log_rep_explicit in *;
           simpl in *; logic_clean.
           unfold log_rep_inner, txns_valid in *; logic_clean.
-          eapply forall_app_l in H17.
+          eapply forall_app_l in H18.
           simpl in *.
-          inversion H17; subst.
-          unfold txn_well_formed in H22; logic_clean.
-          rewrite H21, H0, H4 in *.
+          inversion H18; subst.
+          unfold txn_well_formed in H23; logic_clean.
+          rewrite H22, H0, H5 in *.
           rewrite firstn_app2; eauto.
           rewrite map_length; eauto.
           repeat rewrite map_length; eauto.
@@ -1074,7 +1690,7 @@ Proof.
           {
             apply shift_eq_after.
             intros; lia.
-            intros; rewrite H6; eauto; lia.
+            intros; rewrite H7; eauto; lia.
           }
           {
             unfold sumbool_agree; intros; intuition eauto.
@@ -1082,9 +1698,12 @@ Proof.
             destruct (addr_dec (data_start + y) (data_start + y)); eauto; congruence.
             destruct (addr_dec (data_start + x4) (data_start + y)); eauto; lia.
           }
+          {
+            rewrite H7; simpl; eauto.
+          }
         }
       }
-      all: try rewrite H4, firstn_app2.
+      all: try rewrite H5, firstn_app2.
       all: try rewrite app_length;
       try rewrite map_length; try lia.
       {
@@ -1093,19 +1712,19 @@ Proof.
       }
       {
         apply Forall_forall; intros.
-        apply in_map_iff in H5; cleanup_no_match.
+        apply in_map_iff in H6; cleanup_no_match.
         eapply_fresh Forall_forall in f; eauto.
         pose proof data_fits_in_disk.
         split; try lia.
       }
       {
-        rewrite H4, app_length, map_length; lia.
+        rewrite H5, app_length, map_length; lia.
       }
     }
     {
       unfold log_rep in *; logic_clean.
       destruct (addr_list_to_blocks_to_addr_list (map (Init.Nat.add data_start) al)).
-      eapply commit_finished in H4; eauto.
+      eapply commit_finished in H5; eauto.
       split_ors; cleanup; try congruence.
       {
         split_ors; cleanup; repeat invert_exec;
@@ -1113,89 +1732,6 @@ Proof.
         {
           right; right; left; unfold cached_log_crash_rep; simpl.
           eexists; intuition eauto.
-          
-          rewrite <- sync_list_upd_batch_set.
-          rewrite <- sync_shift_comm.
-          
-          assert (A: map addr_list (x++[x3]) =
-                     map (map (Init.Nat.add data_start))
-                         (map (map (fun a => a - data_start))
-                              (map addr_list (x++[x3])))). {
-            repeat rewrite map_map; simpl.
-            setoid_rewrite map_ext_in at 2.
-            eauto.
-            intros.
-            rewrite map_map.        
-            setoid_rewrite map_ext_in.
-            apply map_id.
-            intros; simpl.
-            unfold log_rep, log_rep_general, log_rep_explicit,
-            log_rep_inner, txns_valid in *; cleanup.
-            
-            eapply Forall_forall in H13; eauto.
-            unfold txn_well_formed, record_is_valid in H13; logic_clean.
-            eapply Forall_forall in H24; eauto; lia.
-          }
-          rewrite A.
-          repeat rewrite shift_list_upd_batch_set_comm.
-          replace (shift (Init.Nat.add data_start) s2) with (shift (Init.Nat.add data_start) (sync s3)); eauto.
-
-          rewrite <- shift_list_upd_batch_set_comm, <- A.
-          rewrite <- total_mem_map_fst_upd_batch_set.
-          rewrite <- shift_upd_batch_set_comm.
-          
-          repeat rewrite map_app.
-          rewrite list_upd_batch_set_app; simpl.
-          rewrite total_mem_map_fst_sync_noop.
-          repeat rewrite total_mem_map_shift_comm.
-          repeat rewrite total_mem_map_fst_upd_batch_set.
-          repeat rewrite total_mem_map_fst_list_upd_batch_set.
-          rewrite total_mem_map_fst_sync_noop; eauto.
-          
-          unfold log_rep, log_rep_general, log_rep_explicit in *;
-          simpl in *; logic_clean.
-          unfold log_rep_inner, txns_valid in *; logic_clean.
-          eapply forall_app_l in H17.
-          simpl in *.
-          inversion H17; subst.
-          unfold txn_well_formed in H22; logic_clean.
-          rewrite H21, H4, H1 in *.
-          rewrite firstn_app2; eauto.
-          rewrite map_length; eauto.
-          repeat rewrite map_length; eauto.
-          
-          {
-            unfold sumbool_agree; intros; intuition eauto.
-            destruct (addr_dec x2 y); subst.
-            destruct (addr_dec (data_start + y) (data_start + y)); eauto; congruence.
-            destruct (addr_dec (data_start + x2) (data_start + y)); eauto; lia.
-          }
-          {
-            unfold sumbool_agree; intros; intuition eauto.
-            destruct (addr_dec x2 y); subst.
-            destruct (addr_dec (data_start + y) (data_start + y)); eauto; congruence.
-            destruct (addr_dec (data_start + x2) (data_start + y)); eauto; lia.
-          }          
-          {
-            apply shift_eq_after.
-            intros; lia.
-            intros; rewrite H8; eauto; lia.
-          }
-          {
-            unfold sumbool_agree; intros; intuition eauto.
-            destruct (addr_dec x2 y); subst.
-            destruct (addr_dec (data_start + y) (data_start + y)); eauto; congruence.
-            destruct (addr_dec (data_start + x2) (data_start + y)); eauto; lia.
-          }
-        }
-        {
-          eapply write_batch_to_cache_crashed in H5.
-          simpl in *; cleanup.
-          right; right; left; unfold cached_log_crash_rep; simpl.
-          eexists; intuition eauto.
-          
-          rewrite <- sync_list_upd_batch_set.
-          rewrite <- sync_shift_comm.
           
           assert (A: map addr_list (x++[x3]) =
                      map (map (Init.Nat.add data_start))
@@ -1226,7 +1762,6 @@ Proof.
           
           repeat rewrite map_app.
           rewrite list_upd_batch_set_app; simpl.
-          rewrite total_mem_map_fst_sync_noop.
           repeat rewrite total_mem_map_shift_comm.
           repeat rewrite total_mem_map_fst_upd_batch_set.
           repeat rewrite total_mem_map_fst_list_upd_batch_set.
@@ -1239,7 +1774,7 @@ Proof.
           simpl in *.
           inversion H18; subst.
           unfold txn_well_formed in H23; logic_clean.
-          rewrite H22, H4, H1 in *.
+          rewrite H22, H5, H1 in *.
           rewrite firstn_app2; eauto.
           rewrite map_length; eauto.
           repeat rewrite map_length; eauto.
@@ -1259,13 +1794,95 @@ Proof.
           {
             apply shift_eq_after.
             intros; lia.
-            intros; rewrite H8; eauto; lia.
+            intros; rewrite H9; eauto; lia.
           }
           {
             unfold sumbool_agree; intros; intuition eauto.
             destruct (addr_dec x2 y); subst.
             destruct (addr_dec (data_start + y) (data_start + y)); eauto; congruence.
             destruct (addr_dec (data_start + x2) (data_start + y)); eauto; lia.
+          }
+          {
+            rewrite H9; simpl; eauto.
+          }
+        }
+        {
+          eapply write_batch_to_cache_crashed in H6.
+          simpl in *; cleanup.
+          right; right; left; unfold cached_log_crash_rep; simpl.
+          eexists; intuition eauto.
+          
+          assert (A: map addr_list (x++[x3]) =
+                     map (map (Init.Nat.add data_start))
+                         (map (map (fun a => a - data_start))
+                              (map addr_list (x++[x3])))). {
+            repeat rewrite map_map; simpl.
+            setoid_rewrite map_ext_in at 2.
+            eauto.
+            intros.
+            rewrite map_map.        
+            setoid_rewrite map_ext_in.
+            apply map_id.
+            intros; simpl.
+            unfold log_rep, log_rep_general, log_rep_explicit,
+            log_rep_inner, txns_valid in *; cleanup.
+            
+            eapply Forall_forall in H15; eauto.
+            unfold txn_well_formed, record_is_valid in H15; logic_clean.
+            eapply Forall_forall in H26; eauto; lia.
+          }
+          rewrite A.
+          repeat rewrite shift_list_upd_batch_set_comm.
+          replace (shift (Init.Nat.add data_start) s2) with (shift (Init.Nat.add data_start) (sync s3)); eauto.
+
+          rewrite <- shift_list_upd_batch_set_comm, <- A.
+          rewrite <- total_mem_map_fst_upd_batch_set.
+          rewrite <- shift_upd_batch_set_comm.
+          
+          repeat rewrite map_app.
+          rewrite list_upd_batch_set_app; simpl.
+          repeat rewrite total_mem_map_shift_comm.
+          repeat rewrite total_mem_map_fst_upd_batch_set.
+          repeat rewrite total_mem_map_fst_list_upd_batch_set.
+          rewrite total_mem_map_fst_sync_noop; eauto.
+          
+          unfold log_rep, log_rep_general, log_rep_explicit in *;
+          simpl in *; logic_clean.
+          unfold log_rep_inner, txns_valid in *; logic_clean.
+          eapply forall_app_l in H19.
+          simpl in *.
+          inversion H19; subst.
+          unfold txn_well_formed in H24; logic_clean.
+          rewrite H23, H5, H1 in *.
+          rewrite firstn_app2; eauto.
+          rewrite map_length; eauto.
+          repeat rewrite map_length; eauto.
+          
+          {
+            unfold sumbool_agree; intros; intuition eauto.
+            destruct (addr_dec x2 y); subst.
+            destruct (addr_dec (data_start + y) (data_start + y)); eauto; congruence.
+            destruct (addr_dec (data_start + x2) (data_start + y)); eauto; lia.
+          }
+          {
+            unfold sumbool_agree; intros; intuition eauto.
+            destruct (addr_dec x2 y); subst.
+            destruct (addr_dec (data_start + y) (data_start + y)); eauto; congruence.
+            destruct (addr_dec (data_start + x2) (data_start + y)); eauto; lia.
+          }          
+          {
+            apply shift_eq_after.
+            intros; lia.
+            intros; rewrite H9; eauto; lia.
+          }
+          {
+            unfold sumbool_agree; intros; intuition eauto.
+            destruct (addr_dec x2 y); subst.
+            destruct (addr_dec (data_start + y) (data_start + y)); eauto; congruence.
+            destruct (addr_dec (data_start + x2) (data_start + y)); eauto; lia.
+          }
+          {
+            rewrite H9; simpl; eauto.
           }
         }
       }
@@ -1289,7 +1906,7 @@ Proof.
     }
     {
       unfold log_rep in *; logic_clean.
-      eapply commit_finished in H4; eauto.
+      eapply commit_finished in H5; eauto.
       {
         split_ors; cleanup; try congruence.
         repeat cleanup_pairs.
@@ -1307,7 +1924,7 @@ Proof.
              {               
                split_ors; cleanup.
                {
-                 left; unfold cached_log_rep; simpl.
+                 left. unfold cached_log_rep; simpl.
                  eexists; intuition eauto.
                  repeat rewrite total_mem_map_shift_comm.
                  repeat rewrite total_mem_map_fst_list_upd_batch_set.
@@ -1316,32 +1933,22 @@ Proof.
                  rewrite upd_batch_to_list_upd_batch_singleton.
                  setoid_rewrite <- list_upd_batch_app at 2.
                  unfold log_rep_general, log_rep_explicit, log_rep_inner, txns_valid in *; logic_clean.
-                 rewrite <- H9.
+                 rewrite <- H10.
                  erewrite RepImplications.bimap_get_addr_list.
                  4: eauto.
-                 rewrite list_upd_batch_firstn_noop; eauto.
-                 {
-                   apply forall_forall2.
-                   apply Forall_forall; intros.
-                   rewrite <- combine_map in H11.
-                   apply in_map_iff in H11; cleanup.
-                   simpl.
-                   eapply Forall_forall in H10; eauto.
-                   unfold txn_well_formed in H10; logic_clean.
-                   rewrite H13.
-                   apply firstn_length_l; eauto.
-                   lia.
-                   repeat rewrite map_length; eauto.
-                 }
+                 rewrite list_upd_batch_firstn_noop; eauto.                 
+                 eapply log_rep_forall2_txns_length_match; eauto.
                  eauto.
                  rewrite map_length; eauto.
                  unfold log_rep_general, log_rep_explicit, log_rep_inner, txns_valid in *; logic_clean.
-                 rewrite <- H9.                 
+                 rewrite <- H10.                 
                  erewrite RepImplications.bimap_get_addr_list.
                  repeat rewrite firstn_length, map_length; eauto.
                  3: eauto.
                  eauto.
                  rewrite map_length; eauto.
+                 (** Apply log crash being synced  not true *)
+                 admit.
                }
                split_ors; cleanup.
                {
@@ -1352,36 +1959,12 @@ Proof.
                  rewrite total_mem_map_fst_sync_noop.
                  rewrite total_mem_map_fst_list_upd_batch_set.
                  unfold log_rep_general, log_rep_explicit, log_rep_inner, txns_valid in *; logic_clean.
-                 rewrite <- H9.
+                 rewrite <- H10.
                  erewrite RepImplications.bimap_get_addr_list.
                  4: eauto.
-                 rewrite list_upd_batch_noop; eauto.
-                 {
-                   apply forall_forall2.
-                   apply Forall_forall; intros.
-                   rewrite <- combine_map in H11.
-                   apply in_map_iff in H11; cleanup.
-                   simpl.
-                   eapply Forall_forall in H10; eauto.
-                   unfold txn_well_formed in H10; logic_clean.
-                   rewrite H13.
-                   apply firstn_length_l; eauto.
-                   lia.
-                   repeat rewrite map_length; eauto.
-                 }
-                 {
-                   apply forall_forall2.
-                   apply Forall_forall; intros.
-                   rewrite <- combine_map in H11.
-                   apply in_map_iff in H11; cleanup.
-                   simpl.
-                   eapply Forall_forall in H10; eauto.
-                   unfold txn_well_formed in H10; logic_clean.
-                   rewrite H13.
-                   apply firstn_length_l; eauto.
-                   lia.
-                   repeat rewrite map_length; eauto.
-                 }
+                 rewrite TotalMem.list_upd_batch_noop; eauto.
+                 eapply log_rep_forall2_txns_length_match; eauto.
+                 eapply log_rep_forall2_txns_length_match; eauto.
                  eauto.
                  rewrite map_length; eauto.
                }
@@ -1392,8 +1975,6 @@ Proof.
                  eexists; intuition eauto.
                  
                  repeat rewrite total_mem_map_shift_comm.
-                 rewrite <- sync_list_upd_batch_set.
-                 rewrite total_mem_map_fst_sync_noop.
                  repeat rewrite total_mem_map_fst_list_upd_batch_set.
                  rewrite total_mem_map_fst_upd_set.
                  rewrite total_mem_map_fst_sync_noop.
@@ -1402,20 +1983,19 @@ Proof.
                  rewrite upd_list_upd_batch_upd_noop.
                  setoid_rewrite shift_upd_noop.
                  unfold log_rep_general, log_rep_explicit, log_rep_inner, txns_valid in *; simpl in *; logic_clean.
-                 rewrite <- H9.
+                 rewrite <- H10.
                  erewrite RepImplications.bimap_get_addr_list.
                  4: eauto.
-                 rewrite list_upd_batch_noop; eauto.
-
+                 rewrite TotalMem.list_upd_batch_noop; eauto.
                  {
                    apply forall_forall2.
                    apply Forall_forall; intros.
-                   rewrite <- combine_map in H11.
-                   apply in_map_iff in H11; cleanup.
+                   rewrite <- combine_map in H12.
+                   apply in_map_iff in H12; cleanup.
                    simpl.
-                   eapply Forall_forall in H10; eauto.
-                   unfold txn_well_formed in H10; logic_clean.
-                   rewrite H13.
+                   eapply Forall_forall in H11; eauto.
+                   unfold txn_well_formed in H11; logic_clean.
+                   rewrite H14.
                    apply firstn_length_l; eauto.
                    lia.
                    repeat rewrite map_length; eauto.
@@ -1423,12 +2003,12 @@ Proof.
                  {
                    apply forall_forall2.
                    apply Forall_forall; intros.
-                   rewrite <- combine_map in H11.
-                   apply in_map_iff in H11; cleanup.
+                   rewrite <- combine_map in H12.
+                   apply in_map_iff in H12; cleanup.
                    simpl.
-                   eapply Forall_forall in H10; eauto.
-                   unfold txn_well_formed in H10; logic_clean.
-                   rewrite H13.
+                   eapply Forall_forall in H11; eauto.
+                   unfold txn_well_formed in H11; logic_clean.
+                   rewrite H14.
                    apply firstn_length_l; eauto.
                    lia.
                    repeat rewrite map_length; eauto.
@@ -1441,15 +2021,16 @@ Proof.
                    lia.
                  }
                  {                   
-                   unfold log_rep_general, log_rep_explicit, log_rep_inner, txns_valid in *; logic_clean.
+                   unfold log_rep_general, log_rep_explicit,
+                   log_rep_inner, txns_valid in *; logic_clean.
                    apply forall_forall2.
                    apply Forall_forall; intros.
-                   rewrite <- combine_map in H11.
-                   apply in_map_iff in H11; cleanup.
+                   rewrite <- combine_map in H12.
+                   apply in_map_iff in H12; cleanup.
                    simpl.
-                   eapply Forall_forall in H10; eauto.
-                   unfold txn_well_formed in H10; logic_clean.
-                   rewrite H13.
+                   eapply Forall_forall in H11; eauto.
+                   unfold txn_well_formed in H11; logic_clean.
+                   rewrite H14.
                    apply firstn_length_l; eauto.
                    lia.
                    repeat rewrite map_length; eauto.
@@ -1462,7 +2043,7 @@ Proof.
                }
              }
           }
-          eapply apply_log_finished in H3; eauto.
+          eapply apply_log_finished in H4; eauto.
           simpl in *; cleanup.
           repeat cleanup_pairs.
           split_ors; cleanup.
@@ -1486,7 +2067,7 @@ Proof.
           { (** Second commit crashed **)
             simpl in *.
             destruct (addr_list_to_blocks_to_addr_list (map (Init.Nat.add data_start) al)).
-            eapply commit_crashed in H5; eauto.
+            eapply commit_crashed in H6; eauto.
             split_ors; cleanup; 
             simpl in *; repeat cleanup_pairs.
             {
@@ -1508,7 +2089,6 @@ Proof.
             {
               right; left; left; eexists; intuition eauto.
               simpl.
-              rewrite <- sync_shift_comm; simpl.
               rewrite shift_eq_after with (m1:= s2) (m2:= sync
          (upd_set (list_upd_batch_set s1 (map addr_list x) (map data_blocks x)) hdr_block_num
                   (encode_header (update_hdr x0 header_part0)))).
@@ -1522,23 +2102,21 @@ Proof.
               }
               intros; lia.
               intros; apply H2; lia.
+              rewrite H2; simpl; eauto.
             }
             split_ors; cleanup; 
             simpl in *; repeat cleanup_pairs.
             {
               right; left; right; do 2 eexists; intuition eauto.
               simpl.
-              replace (addr_list x1) with (map (Init.Nat.add data_start) al).
-              rewrite <- shift_upd_batch_comm.
-              rewrite <- sync_shift_comm; simpl.
+              replace (addr_list x1) with (map (Init.Nat.add data_start) al).           
+              rewrite shift_upd_batch_set_comm.
               rewrite shift_eq_after with (m1:= s2) (m2:= sync
          (upd_set (list_upd_batch_set s1 (map addr_list x) (map data_blocks x)) hdr_block_num
             (encode_header (update_hdr x0 header_part0)))).
               rewrite <- sync_shift_comm.
               rewrite shift_upd_set_noop.
-              rewrite <- total_mem_map_fst_upd_batch_set.
-              rewrite sync_idempotent.
-              repeat rewrite <- sync_upd_batch_set_comm.
+              rewrite total_mem_map_fst_upd_batch_set.
               repeat rewrite total_mem_map_fst_sync_noop; eauto.              
               {
                 intros; pose proof hdr_before_log.
@@ -1546,7 +2124,7 @@ Proof.
                 lia.
               }
               intros; lia.
-              intros; apply H7; lia.
+              intros; apply H8; lia.
               {
                 unfold sumbool_agree; intros; intuition eauto.
                 destruct (addr_dec x3 y); subst.
@@ -1556,15 +2134,14 @@ Proof.
               {
                 unfold log_crash_rep in *; cleanup.
                 simpl in *.
-                unfold log_rep_inner, txns_valid in H15; cleanup.
-                inversion H18; cleanup.
-                unfold txn_well_formed in H21; simpl in *; cleanup.
+                unfold log_rep_inner, txns_valid in H16; cleanup.
+                inversion H19; cleanup.
+                unfold txn_well_formed in H22; simpl in *; cleanup.
                 rewrite firstn_app2; eauto.
                 rewrite map_length; eauto.
               }
               {
                 simpl.
-                rewrite <- sync_shift_comm; simpl.
                 rewrite shift_eq_after with (m1:= s2) (m2:= sync
          (upd_set (list_upd_batch_set s1 (map addr_list x) (map data_blocks x)) hdr_block_num
             (encode_header (update_hdr x0 header_part0)))).
@@ -1577,15 +2154,15 @@ Proof.
                   lia.
                 }
                 intros; lia.
-                intros; apply H7; lia.
+                intros; apply H8; lia.
               }
+              rewrite H8; simpl; eauto.
              }
             {
               right; right; left; eexists; intuition eauto.
               simpl.
               replace (addr_list x1) with (map (Init.Nat.add data_start) al).
-              rewrite <- shift_upd_batch_comm.
-              rewrite <- sync_shift_comm; simpl.
+              rewrite shift_upd_batch_set_comm.
               rewrite shift_eq_after with (m1:= s2) (m2:= sync
          (sync
             (upd_set (list_upd_batch_set s1 (map addr_list x) (map data_blocks x)) hdr_block_num
@@ -1593,83 +2170,7 @@ Proof.
               rewrite sync_idempotent.
               rewrite <- sync_shift_comm.
               rewrite shift_upd_set_noop.
-              rewrite <- total_mem_map_fst_upd_batch_set.
-              rewrite sync_idempotent.
-              repeat rewrite <- sync_upd_batch_set_comm.
-              repeat rewrite total_mem_map_fst_sync_noop; eauto.              
-              
-              {
-                intros; pose proof hdr_before_log.
-                pose proof data_start_where_log_ends.
-                lia.
-              }
-              intros; lia.
-              intros; apply H7; lia.
-              {
-                unfold sumbool_agree; intros; intuition eauto.
-                destruct (addr_dec x3 y); subst.
-                destruct (addr_dec (data_start + y) (data_start + y)); eauto; congruence.
-                destruct (addr_dec (data_start + x3) (data_start + y)); eauto; lia.
-              }
-              {
-                unfold log_rep, log_rep_general, log_rep_explicit in *; cleanup.
-                simpl in *.
-                unfold log_rep_inner, txns_valid in H12; cleanup.
-                inversion H3; cleanup.
-                unfold txn_well_formed in H26; simpl in *; cleanup.
-                rewrite firstn_app2; eauto.
-                rewrite map_length; eauto.
-              }
-            }
-            all: try rewrite H6, firstn_app2.
-            all: try rewrite app_length;
-            try rewrite map_length; try lia.
-            {
-              apply FinFun.Injective_map_NoDup; eauto.
-              unfold FinFun.Injective; intros; lia.
-            }
-            {
-              apply Forall_forall; intros.
-              apply in_map_iff in H7; cleanup_no_match.
-              eapply_fresh Forall_forall in f; eauto.
-              pose proof data_fits_in_disk.
-              split; try lia.
-            }
-            {
-              rewrite H6, app_length, map_length; lia.
-            }
-          }
-          unfold log_rep in *; logic_clean.
-          destruct (addr_list_to_blocks_to_addr_list (map (Init.Nat.add data_start) al)).
-          eapply commit_finished in H5; eauto.
-          simpl in *; repeat cleanup_pairs; simpl in *.
-          split_ors; cleanup; try congruence; try lia.
-          2: {
-            unfold log_rep_general, log_rep_explicit, log_header_block_rep in *; simpl in *; logic_clean.
-            unfold sync, upd_set in H2.
-            destruct (addr_dec hdr_block_num hdr_block_num); try lia.
-            destruct (list_upd_batch_set s1 (map addr_list x) (map data_blocks x) hdr_block_num); simpl in *;
-            destruct x1; simpl in *; cleanup;
-            rewrite encode_decode_header, app_length in H5; simpl in *;
-            lia.
-          }
-          {
-            right; right; left; unfold cached_log_crash_rep; simpl.
-            eexists; intuition eauto.
-            simpl.
-            replace (addr_list x1) with (map (Init.Nat.add data_start) al).
-            rewrite <- shift_upd_batch_comm.
-            rewrite <- sync_shift_comm; simpl.
-            rewrite shift_eq_after with (m1:= s2) (m2:= sync
-         (sync
-            (upd_set (list_upd_batch_set s1 (map addr_list x) (map data_blocks x)) hdr_block_num
-                     (encode_header (update_hdr x0 header_part0))))).
-              rewrite sync_idempotent.
-              rewrite <- sync_shift_comm.
-              rewrite shift_upd_set_noop.
-              rewrite <- total_mem_map_fst_upd_batch_set.
-              rewrite sync_idempotent.
-              repeat rewrite <- sync_upd_batch_set_comm.
+              rewrite total_mem_map_fst_upd_batch_set.
               repeat rewrite total_mem_map_fst_sync_noop; eauto.              
               
               {
@@ -1681,21 +2182,22 @@ Proof.
               intros; apply H8; lia.
               {
                 unfold sumbool_agree; intros; intuition eauto.
-                destruct (addr_dec x2 y); subst.
+                destruct (addr_dec x3 y); subst.
                 destruct (addr_dec (data_start + y) (data_start + y)); eauto; congruence.
-                destruct (addr_dec (data_start + x2) (data_start + y)); eauto; lia.
+                destruct (addr_dec (data_start + x3) (data_start + y)); eauto; lia.
               }
               {
                 unfold log_rep, log_rep_general, log_rep_explicit in *; cleanup.
                 simpl in *.
-                unfold log_rep_inner, txns_valid in H12; cleanup.
-                inversion H3; cleanup.
-                unfold txn_well_formed in H26; simpl in *; cleanup.
+                unfold log_rep_inner, txns_valid in H13; cleanup.
+                inversion H4; cleanup.
+                unfold txn_well_formed in H27; simpl in *; cleanup.
                 rewrite firstn_app2; eauto.
                 rewrite map_length; eauto.
               }
+              rewrite H8; simpl; eauto.
             }
-            all: try rewrite H6, firstn_app2.
+            all: try rewrite H7, firstn_app2.
             all: try rewrite app_length;
             try rewrite map_length; try lia.
             {
@@ -1704,21 +2206,17 @@ Proof.
             }
             {
               apply Forall_forall; intros.
-              apply in_map_iff in H7; cleanup_no_match.
+              apply in_map_iff in H8; cleanup_no_match.
               eapply_fresh Forall_forall in f; eauto.
               pose proof data_fits_in_disk.
               split; try lia.
             }
             {
-              rewrite H6, app_length, map_length; lia.
+              rewrite H7, app_length, map_length; lia.
             }
-        }
-        {(** write_batch_to_cache_crashed **)
-          eapply apply_log_finished in H5; eauto.
-          simpl in *; cleanup.
+          }
           unfold log_rep in *; logic_clean.
           destruct (addr_list_to_blocks_to_addr_list (map (Init.Nat.add data_start) al)).
-          simpl in *; repeat cleanup_pairs; simpl in *.
           eapply commit_finished in H6; eauto.
           simpl in *; repeat cleanup_pairs; simpl in *.
           split_ors; cleanup; try congruence; try lia.
@@ -1728,19 +2226,15 @@ Proof.
             destruct (addr_dec hdr_block_num hdr_block_num); try lia.
             destruct (list_upd_batch_set s1 (map addr_list x) (map data_blocks x) hdr_block_num); simpl in *;
             destruct x1; simpl in *; cleanup;
-            rewrite encode_decode_header, app_length in H5; simpl in *;
+            rewrite encode_decode_header, app_length in H6; simpl in *;
             lia.
           }
-          eapply write_batch_to_cache_crashed in H1; eauto.
-          simpl in *; cleanup.
-          repeat cleanup_pairs; simpl in *.
           {
             right; right; left; unfold cached_log_crash_rep; simpl.
             eexists; intuition eauto.
             simpl.
             replace (addr_list x1) with (map (Init.Nat.add data_start) al).
-            rewrite <- shift_upd_batch_comm.
-            rewrite <- sync_shift_comm; simpl.
+            rewrite shift_upd_batch_set_comm.
             rewrite shift_eq_after with (m1:= s2) (m2:= sync
          (sync
             (upd_set (list_upd_batch_set s1 (map addr_list x) (map data_blocks x)) hdr_block_num
@@ -1748,9 +2242,7 @@ Proof.
               rewrite sync_idempotent.
               rewrite <- sync_shift_comm.
               rewrite shift_upd_set_noop.
-              rewrite <- total_mem_map_fst_upd_batch_set.
-              rewrite sync_idempotent.
-              repeat rewrite <- sync_upd_batch_set_comm.
+              rewrite total_mem_map_fst_upd_batch_set.
               repeat rewrite total_mem_map_fst_sync_noop; eauto.              
               
               {
@@ -1762,6 +2254,85 @@ Proof.
               intros; apply H9; lia.
               {
                 unfold sumbool_agree; intros; intuition eauto.
+                destruct (addr_dec x2 y); subst.
+                destruct (addr_dec (data_start + y) (data_start + y)); eauto; congruence.
+                destruct (addr_dec (data_start + x2) (data_start + y)); eauto; lia.
+              }
+              {
+                unfold log_rep, log_rep_general, log_rep_explicit in *; cleanup.
+                simpl in *.
+                unfold log_rep_inner, txns_valid in H13; cleanup.
+                inversion H4; cleanup.
+                unfold txn_well_formed in H27; simpl in *; cleanup.
+                rewrite firstn_app2; eauto.
+                rewrite map_length; eauto.
+              }
+              rewrite H9; simpl; eauto.
+            }
+            all: try rewrite H7, firstn_app2.
+            all: try rewrite app_length;
+            try rewrite map_length; try lia.
+            {
+              apply FinFun.Injective_map_NoDup; eauto.
+              unfold FinFun.Injective; intros; lia.
+            }
+            {
+              apply Forall_forall; intros.
+              apply in_map_iff in H8; cleanup_no_match.
+              eapply_fresh Forall_forall in f; eauto.
+              pose proof data_fits_in_disk.
+              split; try lia.
+            }
+            {
+              rewrite H7, app_length, map_length; lia.
+            }
+        }
+        {(** write_batch_to_cache_crashed **)
+          eapply apply_log_finished in H6; eauto.
+          simpl in *; cleanup.
+          unfold log_rep in *; logic_clean.
+          destruct (addr_list_to_blocks_to_addr_list (map (Init.Nat.add data_start) al)).
+          simpl in *; repeat cleanup_pairs; simpl in *.
+          eapply commit_finished in H7; eauto.
+          simpl in *; repeat cleanup_pairs; simpl in *.
+          split_ors; cleanup; try congruence; try lia.
+          2: {
+            unfold log_rep_general, log_rep_explicit, log_header_block_rep in *; simpl in *; logic_clean.
+            unfold sync, upd_set in H2.
+            destruct (addr_dec hdr_block_num hdr_block_num); try lia.
+            destruct (list_upd_batch_set s1 (map addr_list x) (map data_blocks x) hdr_block_num); simpl in *;
+            destruct x1; simpl in *; cleanup;
+            rewrite encode_decode_header, app_length in H6; simpl in *;
+            lia.
+          }
+          eapply write_batch_to_cache_crashed in H1; eauto.
+          simpl in *; cleanup.
+          repeat cleanup_pairs; simpl in *.
+          {
+            right; right; left; unfold cached_log_crash_rep; simpl.
+            eexists; intuition eauto.
+            simpl.
+            replace (addr_list x1) with (map (Init.Nat.add data_start) al).
+            rewrite shift_upd_batch_set_comm.
+            rewrite shift_eq_after with (m1:= s2) (m2:= sync
+         (sync
+            (upd_set (list_upd_batch_set s1 (map addr_list x) (map data_blocks x)) hdr_block_num
+                     (encode_header (update_hdr x0 header_part0))))).
+              rewrite sync_idempotent.
+              rewrite <- sync_shift_comm.
+              rewrite shift_upd_set_noop.
+              rewrite total_mem_map_fst_upd_batch_set.
+              repeat rewrite total_mem_map_fst_sync_noop; eauto.              
+              
+              {
+                intros; pose proof hdr_before_log.
+                pose proof data_start_where_log_ends.
+                lia.
+              }
+              intros; lia.
+              intros; apply H10; lia.
+              {
+                unfold sumbool_agree; intros; intuition eauto.
                 destruct (addr_dec x5 y); subst.
                 destruct (addr_dec (data_start + y) (data_start + y)); eauto; congruence.
                 destruct (addr_dec (data_start + x5) (data_start + y)); eauto; lia.
@@ -1769,14 +2340,15 @@ Proof.
               {
                 unfold log_rep, log_rep_general, log_rep_explicit in *; cleanup.
                 simpl in *.
-                unfold log_rep_inner, txns_valid in H12; cleanup.
+                unfold log_rep_inner, txns_valid in H13; cleanup.
                 inversion H1; cleanup.
-                unfold txn_well_formed in H26; simpl in *; cleanup.
+                unfold txn_well_formed in H27; simpl in *; cleanup.
                 rewrite firstn_app2; eauto.
                 rewrite map_length; eauto.
               }
+              rewrite H10; simpl; eauto.
             }
-            all: try rewrite H8, firstn_app2.
+            all: try rewrite H9, firstn_app2.
             all: try rewrite app_length;
             try rewrite map_length; try lia.
             {
@@ -1791,7 +2363,7 @@ Proof.
               split; try lia.
             }
             {
-              rewrite H8, app_length, map_length; lia.
+              rewrite H9, app_length, map_length; lia.
             }
         }
       }
@@ -1818,7 +2390,7 @@ Proof.
   all: try solve [left; eexists; intuition eauto].
   Unshelve.
   apply value0.
-Qed.
+Admitted.
 
 
   
